proven a bunch of callset_translate_ lemmas

From10To20/Translate.v
@@ -1,6 +1,6 @@
 From Coq Require Import String ZArith.
 From Vyper Require Import Config.
-From Vyper Require L10.AST L20.AST L10.Interpret.
+From Vyper Require L10.AST L20.AST L10.Interpret L20.Interpret.
 
 Section Translate.
 
@@ -83,7 +83,7 @@ Fixpoint translate_stmt (s: L10.AST.stmt)
    := fix translate_stmt_list (l: list L10.AST.stmt)
       := match l with
          | nil => L20.AST.SmallStmt L20.AST.Pass
-         | (h :: nil)%list => translate_stmt h
+         (* | (h :: nil)%list => translate_stmt h      <- this case makes stuff too complicated *)
          | (L10.AST.LocalVarDecl name maybe_init :: t)%list =>
              L20.AST.LocalVarDecl name
                                   match maybe_init with
@@ -128,7 +128,6 @@ Fixpoint translate_stmt_list (l: list L10.AST.stmt)
 : L20.AST.stmt
 := match l with
    | nil => L20.AST.SmallStmt L20.AST.Pass
-   | (h :: nil)%list => translate_stmt h
    | (L10.AST.LocalVarDecl name maybe_init :: t)%list =>
        L20.AST.LocalVarDecl name
                             match maybe_init with
@@ -140,6 +139,320 @@ Fixpoint translate_stmt_list (l: list L10.AST.stmt)
                                         (translate_stmt_list t)
    end.
 
+Definition translate_decl (d: L10.AST.decl)
+: L20.AST.decl
+:= match d with
+   | L10.AST.StorageVarDecl name => L20.AST.StorageVarDecl name
+   | L10.AST.FunDecl name arg_names body =>
+       L20.AST.FunDecl name arg_names (translate_stmt_list body)
+   end.
+
 End Translate.
 
+Fixpoint decl_names {C: VyperConfig} (decls: list L10.AST.decl)
+:= List.map L10.AST.decl_name decls.
+
+Definition decl_set {C: VyperConfig} (decls: list L10.AST.decl)
+: string_set
+:= let _ := string_set_impl in FSet.from_list (decl_names decls).
+
+(* superceded by translate_calldag *)
+Definition translate_decl_list {C: VyperConfig} (d: list L10.AST.decl)
+: list L20.AST.decl
+:= let f := decl_set d in
+   let is_private_call (name: string) := let _ := string_set_impl in FSet.has f name in
+   List.map (translate_decl is_private_call) d.
+
+(** After translation, the callsets get filtered by [is_private_call] predicate. *)
+Lemma callset_translate_expr {C: VyperConfig}
+                             (is_private_call: string -> bool)
+                             (e: L10.AST.expr)
+                             (x: string):
+  let _ := string_set_impl in
+  FSet.has (L20.Callset.expr_callset (translate_expr is_private_call e)) x
+   =
+  (FSet.has (L10.Callset.expr_callset e) x && is_private_call x)%bool.
+Proof.
+cbn.
+induction e using L10.AST.expr_ind'; intros; cbn;
+  try repeat rewrite FSet.union_ok;
+  try rewrite FSet.empty_ok;
+  try rewrite IHe1; try rewrite IHe2; try rewrite IHe3;
+  try repeat rewrite<- Bool.andb_orb_distrib_l;
+  try easy.
+(* only the PrivateOrBuiltinCall case remains *)
+rewrite FSet.add_ok.
+remember (is_private_call name) as priv_name. destruct priv_name; cbn.
+{
+  rewrite FSet.add_ok.
+  destruct (string_dec name x). { subst. now rewrite<- Heqpriv_name. }
+  induction args. { now rewrite FSet.empty_ok. }
+  cbn.
+  repeat rewrite FSet.union_ok.
+  rewrite (List.Forall_inv H).
+  rewrite IHargs by apply (List.Forall_inv_tail H).
+  (* clear H IHargs Heqpriv_name n.
+  remember (FSet.has (L10.Callset.expr_callset a) x) as p. clear Heqp.
+  remember (FSet.has (_ args) x) as q. clear Heqq.
+  remember (is_private_call x) as r. clear Heqr. *)
+  symmetry.
+  apply Bool.andb_orb_distrib_l.
+}
+(* a builtin call *)
+destruct (string_dec name x).
+{
+  subst. rewrite<- Heqpriv_name. cbn.
+  induction args. { apply FSet.empty_ok. }
+  rewrite FSet.union_ok.
+  rewrite IHargs by apply (List.Forall_inv_tail H).
+  rewrite (List.Forall_inv H).
+  rewrite<- Heqpriv_name.
+  rewrite Bool.andb_false_r.
+  trivial.
+}
+(* name <> x *)
+induction args. { now rewrite FSet.empty_ok. }
+repeat rewrite FSet.union_ok.
+rewrite IHargs by apply (List.Forall_inv_tail H).
+rewrite (List.Forall_inv H).
+symmetry.
+apply Bool.andb_orb_distrib_l.
+Qed.
+
+Lemma callset_translate_small_stmt {C: VyperConfig}
+                                   (is_private_call: string -> bool)
+                                   (ss: L10.AST.small_stmt)
+                                   (x: string):
+  let _ := string_set_impl in
+  FSet.has (L20.Callset.stmt_callset (translate_small_stmt is_private_call ss)) x
+   =
+  (FSet.has (L10.Callset.small_stmt_callset ss) x && is_private_call x)%bool.
+Proof.
+destruct ss; cbn;
+  repeat rewrite FSet.union_ok;
+  try rewrite FSet.empty_ok;
+  repeat rewrite callset_translate_expr;
+  try easy.
+{ (* return *)
+  destruct result. { cbn. apply callset_translate_expr. }
+  rewrite FSet.empty_ok. cbn. apply FSet.empty_ok.
+}
+{ (* assert *)
+  destruct error.
+  {
+    rewrite callset_translate_expr. cbn.
+    rewrite FSet.union_ok.
+    symmetry. apply Bool.andb_orb_distrib_l.
+  }
+  cbn. rewrite FSet.empty_ok. apply Bool.orb_false_r.
+}
+(* binop assign *)
+destruct lhs; cbn; rewrite FSet.empty_ok; easy.
+Qed.
+
+(* The callsets of statement lists behave normally ASSUMING that each statement behaves normally.
+   We'll get rid of this assumption later.
+ *)
+Lemma callset_translate_stmt_list_aux {C: VyperConfig}
+                                      (is_private_call: string -> bool)
+                                      (l: list L10.AST.stmt)
+                                      (x: string)
+                 (Ok: let _ := string_set_impl in
+                      List.Forall
+                        (fun s : L10.AST.stmt =>
+                          FSet.has (Callset.stmt_callset (translate_stmt is_private_call s)) x
+                           =
+                         (FSet.has (L10.Callset.stmt_callset s) x && is_private_call x)%bool) 
+                        l):
+  let _ := string_set_impl in
+  FSet.has (L20.Callset.stmt_callset (translate_stmt_list is_private_call l)) x
+   =
+  (FSet.has (L10.Callset.stmt_list_callset l) x && is_private_call x)%bool.
+Proof.
+cbn in *. induction l. { cbn. now repeat rewrite FSet.empty_ok. }
+cbn. rewrite FSet.union_ok.
+assert (Inv := List.Forall_inv Ok).
+assert (IH := (IHl (List.Forall_inv_tail Ok))).
+assert (SemicolonRewrite:
+          forall (a b: L20.AST.stmt),
+            L20.Callset.stmt_callset (L20.AST.Semicolon a b)
+             =
+            let _ := string_set_impl in
+            FSet.union (L20.Callset.stmt_callset a) (L20.Callset.stmt_callset b)).
+{ easy. }
+assert (LocalVarDeclRewrite:
+          forall name init body,
+            L20.Callset.stmt_callset
+             (L20.AST.LocalVarDecl name init body)
+             =
+            let _ := string_set_impl in
+            FSet.union (L20.Callset.expr_callset init)
+                       (L20.Callset.stmt_callset body)).
+{ easy. }
+destruct a, l; try destruct init;
+  try rewrite SemicolonRewrite;
+  try rewrite LocalVarDeclRewrite;
+  try rewrite FSet.union_ok;
+  try rewrite callset_translate_expr;
+  try rewrite Inv; try rewrite IH;
+  try (symmetry; apply Bool.andb_orb_distrib_l);
+  try (cbn; rewrite FSet.empty_ok; rewrite Bool.orb_false_r);
+  try easy.
+(* remaining case: LocalVarDecl without init *)
+cbn. now repeat rewrite FSet.empty_ok.
+Qed.
+
+Lemma callset_translate_stmt {C: VyperConfig}
+                             (is_private_call: string -> bool)
+                             (s: L10.AST.stmt)
+                             (x: string):
+  let _ := string_set_impl in
+  FSet.has (L20.Callset.stmt_callset (translate_stmt is_private_call s)) x
+   =
+  (FSet.has (L10.Callset.stmt_callset s) x && is_private_call x)%bool.
+Proof.
+cbn.
+induction s using L10.AST.stmt_ind'; intros; cbn;
+  repeat rewrite FSet.union_ok.
+{ (* SmallStmt *) apply callset_translate_small_stmt. }
+{ (* LocalVarDecl *)
+  destruct init; rewrite FSet.empty_ok; rewrite Bool.orb_false_r.
+  { apply callset_translate_expr. }
+  cbn. apply FSet.empty_ok.
+}
+{ (* If *)
+  assert (OkYes := callset_translate_stmt_list_aux is_private_call yes x H).
+  destruct no; repeat rewrite FSet.union_ok; rewrite callset_translate_expr; cbn.
+  {
+    assert (OkNo := callset_translate_stmt_list_aux is_private_call l x H0).
+    unfold translate_stmt_list in OkYes. rewrite OkYes.
+    unfold translate_stmt_list in OkNo. rewrite OkNo.
+    repeat rewrite Bool.andb_orb_distrib_l.
+    trivial.
+  }
+  unfold translate_stmt_list in OkYes. rewrite OkYes.
+  rewrite Bool.andb_orb_distrib_l. rewrite FSet.empty_ok.
+  rewrite Bool.orb_false_r.
+  trivial.
+}
+{ (* FixedRangeLoop *)
+  assert (OkBody := callset_translate_stmt_list_aux is_private_call body x H).
+  unfold translate_stmt_list in OkBody. rewrite OkBody.
+  rewrite FSet.empty_ok. rewrite Bool.orb_false_l.
+  trivial.
+}
+(* FixedCountLoop *)
+assert (OkBody := callset_translate_stmt_list_aux is_private_call body x H).
+unfold translate_stmt_list in OkBody. rewrite OkBody.
+rewrite Bool.andb_orb_distrib_l.
+now rewrite callset_translate_expr.
+Qed.
+
+Lemma callset_translate_stmt_list {C: VyperConfig}
+                                  (is_private_call: string -> bool)
+                                  (l: list L10.AST.stmt)
+                                  (x: string):
+  let _ := string_set_impl in
+  FSet.has (L20.Callset.stmt_callset (translate_stmt_list is_private_call l)) x
+   =
+  (FSet.has (L10.Callset.stmt_list_callset l) x && is_private_call x)%bool.
+Proof.
+apply callset_translate_stmt_list_aux.
+induction l. { easy. }
+refine (List.Forall_cons _ _ IHl).
+apply callset_translate_stmt.
+Qed.
+
+Lemma callset_translate_decl {C: VyperConfig}
+                             (is_private_call: string -> bool)
+                             (d: L10.AST.decl)
+                             (x: string):
+  let _ := string_set_impl in
+  FSet.has (L20.Callset.decl_callset (translate_decl is_private_call d)) x
+   =
+  (FSet.has (L10.Callset.decl_callset d) x && is_private_call x)%bool.
+Proof.
+destruct d; cbn. { now rewrite FSet.empty_ok. }
+apply callset_translate_stmt_list.
+Qed.
+
+(*************************************************************************************************)
+
+Lemma translate_calldag_helper {C: VyperConfig}
+                               (cd: L10.Interpret.calldag):
+  let is_private_call (name: string)
+   := match L10.Interpret.cd_declmap cd name with
+      | Some _ => true
+      | _ => false
+      end 
+  in forall name: string,
+       match
+          match L10.Interpret.cd_declmap cd name with
+          | Some f => Some (translate_decl is_private_call f)
+          | None => None
+          end
+       with
+       | Some decl =>
+           match L10.Interpret.cd_depthmap cd name with
+           | Some x =>
+               let _ := string_set_impl in
+               FSet.for_all (Callset.decl_callset decl)
+                 (fun callee : string =>
+                  match L10.Interpret.cd_depthmap cd callee with
+                  | Some y => y <? x
+                  | None => false
+                  end) = true
+           | None => False
+           end
+       | None => True
+       end.
+Proof.
+intros is_private_call name.
+assert (D := L10.Interpret.cd_depthmap_ok cd name).
+cbn.
+remember (L10.Interpret.cd_declmap cd name) as maybe_f. destruct maybe_f. 2:easy.
+destruct (L10.Interpret.cd_depthmap cd name). 2:easy.
+rewrite FSet.for_all_ok in *. intros x H.
+rewrite callset_translate_decl in H.
+apply Bool.andb_true_iff in H.
+assert (Q := D x (proj1 H)). clear D.
+destruct (L10.Interpret.cd_depthmap cd x). 2:easy.
+destruct n; rewrite Nat.ltb_lt in Q. { now apply Nat.nlt_0_r in Q. }
+rewrite Nat.leb_le.
+apply Nat.lt_succ_r. exact Q.
+Qed.
+
+
+(* XXX This is inefficient since functions are translated at each lookup.
+   It's better to rebuild the calldag.
+ *)
+Definition translate_calldag {C: VyperConfig} (cd: L10.Interpret.calldag)
+:= let is_private_call (name: string)
+   := match L10.Interpret.cd_declmap cd name with
+      | Some _ => true
+      | _ => false
+      end
+   in {| L20.Interpret.cd_declmap (name: string) :=
+              match L10.Interpret.cd_declmap cd name with
+              | Some f => Some (translate_decl is_private_call f)
+              | None => None
+              end
+       ; L20.Interpret.cd_depthmap := L10.Interpret.cd_depthmap cd
+       ; L20.Interpret.cd_depthmap_ok := translate_calldag_helper cd
+      |}.
+
 (***************************************************************************************************)
+
+(*
+Theorem translate_ok {C: VyperConfig}
+                     (builtins: string -> option L10.Interpret.builtin)
+                     (cd: L10.Interpret.calldag)
+                     (fun_name: string)
+                     (world: world_state)
+                     (arg_values: list uint256):
+  L20.Interpret.interpret builtins (translate_calldag cd) fun_name world arg_values
+   =
+  L10.Interpret.interpret builtins cd fun_name world arg_values.
+Proof.
+unfold L10.Interpret.interpret.
+unfold L20.Interpret.interpret. *)
