L10/AST.v
@@ -51,6 +51,45 @@ Inductive expr
  | LogicalOr (a b: expr)
  | PrivateOrBuiltinCall (name: string) (args: list expr).
 
+(* Coq derives wrong induction principle because lists are present. Here's the correct one. *)
+Fixpoint expr_ind' (P: expr -> Prop)
+                   (HConst: forall val, P (Const val))
+                   (HLocalVar: forall name, P (LocalVar name))
+                   (HStorageVar: forall name, P (StorageVar name))
+                   (HUnOp: forall op a, P a -> P (UnOp op a))
+                   (HBinOp: forall op a b, P a -> P b -> P (BinOp op a b))
+                   (HIf: forall cond yes no: expr,
+                           P cond -> P yes -> P no -> P (IfThenElse cond yes no))
+                   (HAnd: forall a b, P a -> P b -> P (LogicalAnd a b))
+                   (HOr:  forall a b, P a -> P b -> P (LogicalOr  a b))
+                   (HCall: forall name args,
+                        Forall P args -> P (PrivateOrBuiltinCall name args))
+                   (e: expr)
+{struct e}
+: P e
+:= let ind := expr_ind' P HConst HLocalVar HStorageVar HUnOp HBinOp HIf HAnd HOr HCall in
+   match e with
+   | Const val => HConst val
+   | LocalVar name => HLocalVar name
+   | StorageVar name => HStorageVar name
+   | UnOp op a => HUnOp op a (ind a)
+   | BinOp op a b => HBinOp op a b (ind a) (ind b)
+   | IfThenElse cond yes no => HIf cond yes no (ind cond) (ind yes) (ind no)
+   | LogicalAnd a b => HAnd a b (ind a) (ind b)
+   | LogicalOr a b => HOr a b (ind a) (ind b)
+   | PrivateOrBuiltinCall name args =>
+      HCall name args
+        ((fix expr_list_ind (l: list expr)
+          : Forall P l
+          := match l with
+             | nil => Forall_nil P
+             | cons h t => Forall_cons h (ind h) (expr_list_ind t)
+             end)
+          args)
+   end.
+
+
+
 (** "Small statement" is a term used in Python grammar, also in rust-vyper grammar.
     Here we don't count local variable declarations as small statements.
  *)
@@ -69,11 +108,49 @@ Inductive small_stmt
 
 
 Inductive stmt
-:= SmallStmt (s: small_stmt)
+:= SmallStmt (ss: small_stmt)
  | LocalVarDecl (name: string) (init: option expr)
  | IfElseStmt (cond: expr) (yes: list stmt) (no: option (list stmt))
  | FixedRangeLoop (var: string) (start: option uint256) (stop: uint256) (body: list stmt)
  | FixedCountLoop (var: string) (start: expr) (count: uint256) (body: list stmt).
+
+Fixpoint stmt_ind' (P: stmt -> Prop)
+                   (HSmall: forall ss, P (SmallStmt ss))
+                   (HLocalVar: forall name init, P (LocalVarDecl name init))
+                   (HIf: forall cond yes no,
+                           Forall P yes 
+                            ->
+                           match no with
+                           | Some else_branch => Forall P else_branch
+                           | None => True
+                           end 
+                            ->
+                           P (IfElseStmt cond yes no))
+                   (HRangeLoop: forall var start stop body,
+                                  Forall P body 
+                                   ->
+                                  P (FixedRangeLoop var start stop body))
+                   (HCountLoop: forall var start count body,
+                                  Forall P body 
+                                   ->
+                                  P (FixedCountLoop var start count body))
+                   (s: stmt)
+: P s
+:= let ind := stmt_ind' P HSmall HLocalVar HIf HRangeLoop HCountLoop in
+   let fix stmt_list_ind (l: list stmt)
+       : Forall P l
+       := match l with
+          | nil => Forall_nil P
+          | cons h t => Forall_cons h (ind h) (stmt_list_ind t)
+          end
+   in match s with
+      | SmallStmt ss => HSmall ss
+      | LocalVarDecl name init => HLocalVar name init
+      | IfElseStmt cond yes (Some no) => HIf cond yes (Some no) (stmt_list_ind yes) (stmt_list_ind no)
+      | IfElseStmt cond yes None => HIf cond yes None (stmt_list_ind yes) I
+      | FixedRangeLoop var start stop body => HRangeLoop var start stop body (stmt_list_ind body)
+      | FixedCountLoop var start stop body => HCountLoop var start stop body (stmt_list_ind body)
+      end.
 
 Inductive decl
 := (* ImportDecl
