L20/AST.v
@@ -19,6 +19,45 @@ Inductive expr
  | PrivateCall (name: string) (args: list expr)
  | BuiltinCall (name: string) (args: list expr).
 
+Fixpoint expr_ind' (P: expr -> Prop)
+                   (HConst: forall val, P (Const val))
+                   (HLocalVar: forall name, P (LocalVar name))
+                   (HStorageVar: forall name, P (StorageVar name))
+                   (HUnOp: forall op a, P a -> P (UnOp op a))
+                   (HBinOp: forall op a b, P a -> P b -> P (BinOp op a b))
+                   (HIf: forall cond yes no: expr,
+                           P cond -> P yes -> P no -> P (IfThenElse cond yes no))
+                   (HAnd: forall a b, P a -> P b -> P (LogicalAnd a b))
+                   (HOr:  forall a b, P a -> P b -> P (LogicalOr  a b))
+                   (HPrivateCall: forall name args,
+                        Forall P args -> P (PrivateCall name args))
+                   (HBuiltinCall: forall name args,
+                        Forall P args -> P (BuiltinCall name args))
+                   (e: expr)
+{struct e}
+: P e
+:= let ind := expr_ind' P HConst HLocalVar HStorageVar 
+                        HUnOp HBinOp HIf HAnd HOr 
+                        HPrivateCall HBuiltinCall
+    in let fix expr_list_ind (l: list expr)
+       : Forall P l
+       := match l with
+          | nil => Forall_nil P
+          | cons h t => Forall_cons h (ind h) (expr_list_ind t)
+          end
+    in match e with
+     | Const val => HConst val
+     | LocalVar name => HLocalVar name
+     | StorageVar name => HStorageVar name
+     | UnOp op a => HUnOp op a (ind a)
+     | BinOp op a b => HBinOp op a b (ind a) (ind b)
+     | IfThenElse cond yes no => HIf cond yes no (ind cond) (ind yes) (ind no)
+     | LogicalAnd a b => HAnd a b (ind a) (ind b)
+     | LogicalOr a b => HOr a b (ind a) (ind b)
+     | PrivateCall name args => HPrivateCall name args (expr_list_ind args)
+     | BuiltinCall name args => HBuiltinCall name args (expr_list_ind args)
+     end.
+
 (** "Small statement" is a term used in Python grammar, also in rust-vyper grammar.
     Here we don't count local variable declarations as small statements.
  *)
